---
id: 1729670681-mipt-ДУ-seminar-23-10-24
aliases:
  - MIPT ДУ seminar 23-10-24
tags: []
---

# MIPT ДУ seminar 23-10-24

[[1729669731-ДУ-с-постоянными-коэффицентами|ДУ с постоянными коэффицентами]]

## Exercises

### 8.3.  ${y}^{''} + 3 {y}^{'} + 2y = 0$
$$
\alignleft{
y = e^{\alpha x} \implies \\
\alpha_1 = -1,\quad \alpha_2 = -2 \\
}
$$

### 8.7.  ${y}^{''} - 6{y}^{'} + 18y = 0$ 
$$
\alignleft{
y = e^{\alpha x} \implies \\
\alpha_1 = 3 + 3i,\quad \alpha_2 = 3 - 3i \\
y_1 = \exp{3x} \cos{3x},\quad y_2 = \exp{3x} \sin{3x} \\
y = C_1 y_1 + C_2 y_2 = \exp{3x} (C_1 \cos{3x} + C_2 \sin{3x}) \\
}
$$

### 8.12.  ${y}^{''} - 6{y}^{'} + 9y = 0$ 
$$
\alignleft{
y = e^{\alpha x} \implies \\
\alpha_{1,2} = 3 \\
y_1 = \exp{3x},\quad y_2 = \exp{3x} x \\
y = C_1 y_1 + C_2 y_2 = \exp{3x} (C_1 + C_2 x) \\
}
$$

### 8.23.  ${y}^{(4)} - {y}^{(3)} + 2y^{(1)} = 0$ 
$$
\alignleft{
y = e^{\alpha x} \implies \\
\alpha_{1} = 0,\quad \alpha_{2} = -1,\quad
\alpha_{3} = 1 + i,\quad \alpha_{4} = 1 - i \\
y_1 = 1, \quad y_2 = \exp{-x},\quad
y_3 = \exp{x}\cos{x},\quad y_4 = \exp{x}\sin{x} \\
y = \sum_{}^{}{C_i y_i} \\
}
$$

### 8.31.  ${y}^{(4)} + 6{y}^{(3)} + 12y^{(2)} + 8y^{(1)} = 0$ 
$$
\alignleft{
y = e^{\alpha x} \implies \\
\alpha_{1} = 0,\quad \alpha_{2,3,4} = -2 \\
y_1 = 1, \quad
y_2 = \exp{-2x},\quad
y_3 = \exp{-2x} x,\quad
y_4 = \exp{-2x} x^2,\quad
y_3 = \exp{x}\cos{x},\quad y_4 = \exp{x}\sin{x} \\
y = \sum_{}^{}{C_i y_i} \\
}
$$

### 8.47.  ${y}^{(2)} + 4{y}^{} = 4x\ \exp{-2x} - \sin{2x}$ 
$$
\alignleft{
y_o:\\
y = e^{\alpha x} \implies \\
\alpha_{1} = 2i,\quad \alpha_{2} = -2i \\
y_1 = \cos{2x}, \quad
y_2 = \sin{2x} \\
y_o = C_1 \cos{2x} + C_2 \sin{2x} \\
y_c: \\
y_{c_1} = (ax + b) \exp{-2x} x^s,\quad s = 0 \\
a = \frac{1}{2},\quad b = \frac{1}{4} \\
y_{c_1} = \frac{1}{2}(x + \frac{1}{2}) \exp{-2x} \\
\sin{2x} = \frac{\exp{2xi} - \exp{-2xi}}{2i} \\
y_{c_2} = a \sin{2x} \cdot x + b \cos{2x} \cdot x \\
a = 0,\quad b = -\frac{1}{4} \\
y_{c_2} = -\frac{1}{4} x \cos{2x}
}
$$
$$
y = C_1 \cos{2x} + C_2 \sin{2x} + \frac{1}{2}(x + \frac{1}{2}) \exp{-2x} -\frac{1}{4} x \cos{2x}
$$
