---
id: 1732694753-mipt-ДУ-seminar-27-11-24
aliases:
  - MIPT ДУ seminar 27-11-24
tags: []
---

# MIPT ДУ seminar 27-11-24
![[1732694805.png]]
![[1732694821.png]]
![[1732694829.png]]
## 11.128
$$
\Gather{
x(0) = c_1, \quad y(0) = c_2 \\
A = \Pmatrix{
2 & -3 \\
3 & 2
}
}
$$
$$
\alignleft{
\lambda = 2 \pm 3i \\
h_1 = \Pmatrix{1 \\ i} \\
h_2 = \Pmatrix{1 \\ -i} \\
\tilde{A} = \Pmatrix{
2 - 3i & 0 \\
0 & 2 + 3i
} \\
e^{\tilde{A} t} = \Pmatrix{
e^{(2 - 3i)t} & 0 \\
0 & e^{(2 + 3i)t}
} = e^{2t} \Pmatrix{
e^{- 3it} & 0 \\
0 & e^{3it}
} \\
S = \Pmatrix{
1 & 1 \\
i & -i
} \\
S^{-1} = \frac{1}{2} \Pmatrix{
1 & -i \\
1 & i \\
} \\
e^{At} =- S e^{\tilde{A}t} S^{-1} = 
e^{2t} \Pmatrix{
\cos{3t} & -\sin{3t} \\
\cos{3t} & \sin{3t} \\
}
}
$$
## 11.124
$$
\Cases{
\dot{x} = 2x - y \\
\dot{y} = x + 4y
}
$$
$$
\alignleft{
A = \Pmatrix{
2 & -1 \\
1 & 4
} \\
\lambda_{1,2} = 3 \\
h_1 = \Pmatrix{1 \\ -1} \\
(A - \lambda E) h_2 = h_1 \\
h_2 = \Pmatrix{-1 \\ 0} + C h_1, \quad C = 0 \\
e^{\tilde{A}t} = e^{3t} \Pmatrix{
1 & t \\
0 & 1
}
S = \Pmatrix{
1 & -1 \\
-1 & 0
} \\
S^{-1} = \Pmatrix{
0 & -1 \\
-1 & -1
} \\
e^{At} = S e^{\tilde{A}t} S^{-1} = 
e^{3t} \Pmatrix{
1-t & -t \\
t & 1+t
} \\
x = e^{At} \Pmatrix{2 \\ 2} = 2 e^{3t} \Pmatrix{4t \\ 2t + 1}
}
$$
## 4*
$$
\det{e^{A}} = e^{\tr{A}}
$$
$$
\alignleft{
\det{e^{A}} = \det{S e^{\tilde{A}} S^{-1}} = \det{e^{\tilde{A}}} = e^{\tr{\tilde{A}}} = e^{\tr{A}}
}
$$
## 2
![[1732697539.png]]
![[1732697550.png]]
![[1732697560.png]]
## 3
![[1732697520.png]]
$$
\alignleft{
A = \mathrm{diag}(2, 2, 2, 3, 3) \\
B = \Pmatrix{
0 & 1 && ... \\
0 & 0 & 1 & ... \\
0 & ... &
} \\
e^{{A}^{'}} = e^{A + B} = e^{A} e^{B} \\
e^{A} = \mathrm{diag}(e^{2}, e^{2}, e^{2}, e^{3}, e^{3}) \\
B^2 = \Pmatrix{
0 & 0 & 1 & 0 & ... \\
0 && ... && 0 \\
&& \dots \\
0 && ... && 0 \\
} \\
B^3 = 0 \\
e^{B} = E + B + \frac{B^2}{2} \\
}
$$
## $\Phi 824$
 $$
\Cases{
\ddot{x} + 4 \dot{x} - 2x - 2 \dot{y} - y = 0 \\
\ddot{x} - 4 \dot{x} - \ddot{y} - 2 \dot{y} + 2y = 0 \\
}
$$
$$
\alignleft{
1 + 2 \implies\\
2x - y = 2 \ddot{x} - \ddot{y} \\
z = 2x - y \\
\ddot{z} = z \\
z = c_1 e^{t} + c_2 e^{-t} \\
\ddot{x} - 4x = -3 c_1 e^{t} + c_2 e^{-t} \\

}
$$
