---
id: 1733298571-преобразование-Лапласа
aliases:
  - преобразование Лапласа
tags: []
---

# преобразование Лапласа
![[1733299687.png]]
## Операционный метод
Пр-во оригиналов
Пр-во отображений
$f(x) = F(p)$
1. $f(x) = 0, \quad x < 0$
2. $f(x)$ непр., конечное число т. разрыва I рода
3. $f(x)$ - ф-ия ограниченного роста:
 $$
\exists M > 0 : \exists \alpha > 0 : \abs{f(x)} \le M e^{\alpha x}
$$
$$
F(p) = \int_0^\infty{e^{-px}f(x) \d x}
$$
$p = u + iv \in \CC$
 $$
\lim_{u \to \infty} F(p) = 0
$$
## Обратное преобразованиех
$$
f(x) = \frac{1}{2\pi i} \int_{u - i \infty}^{u + i \infty}{e^{px} F(p) \d p}
$$
## 8.172
![[1733299819.png]]
$$
\alignleft{
y = F(p) \\
{y}^{'} = p F(p) \\
{y}^{''} = p^2 F(p) - 1 \\
e^{-t} = \frac{1}{p+1} \\
p^2 F(p) - 1 - 3p F(p) + 2 F(p) = \frac{1}{p + 1} \\
F(p) = \frac{1}{6} \frac{1}{p+1} - \frac{3}{2} \frac{1}{p-1} + 
\frac{4}{3} \frac{1}{p - 2} \\
y(t) = \frac{1}{6} e^{-t} - \frac{3}{2} e^{t} + \frac{4}{3} e^{2t}
}
$$
## 8.182
![[1733299853.png]]
$$
\alignleft{
y = F(p) \\
{y}^{'} = p F(p) - f(0) = p F(p) \\
{y}^{''} = p^2 F(p) - {f}^{'}(0) - p f(0) = p^2 F(p) - 1 \\
p^2 F(p) - 1 + 4F(p) = 4(\frac{p}{p^2 + 4} + \frac{2}{p^2 + 4}) \\
F(p) = \frac{p^2 + 4p + 12}{(p^2 + 4)^2} = 
A \frac{p^2 - 4}{p^2 + 4} + B \frac{4p}{(p^2 + 4)^2} + C \frac{p}{p^2 + 4} + 
D \frac{2}{p^2 +4} \\
A(p^2 - 4) + 4Bp + Cp(p^2 + 4) + 2D (p^2 + 4) = p^2 + 4p +12 \\
C = 0, \quad B = 1, \quad A = -1, \quad D = 1 \\
F(p) = (-1) \frac{p^2 - 2^2}{(p^2 + 2^2)^2} + 4 \frac{p}{(p^2 + 2^2)^2} +
2 \frac{1}{p^2 + 2^2} \\
f(t) = -t \cos{2t} + t \sin{2t} + \sin{2t}
}
$$
## 11.189
![[1733300820.png]]
$$
\alignleft{
x = f(p), \quad y = g(p) \\
{x}^{'} = p f(p) - 1, \quad {y}^{'} = p g(p) - 2 \\
e^{2t} = \frac{1}{p - 2} \\
f(p) = \frac{p^2 - 3p + 1}{(p-3)(p-2)^2} = 
A \frac{1}{p-2} + B \frac{1}{(p - 2)^2} + C \frac{1}{p - 3} \\
A = 0, \quad B = 1, \quad C = 1 \\
x = e^{3t} + t e^{2t} \\
g(p) = 
} \\
g(p) = \frac{2}{p - 3} + \frac{1}{(p-2)^2} \\
y = 2 e^{3t} + t e^{2t} \\
$$
## 11.194
![[1733302134.png]]
$$
\alignleft{
x = f(p), \quad y = g(p) \\
{x}^{'} = p f(p), \quad {y}^{'} = p g(p) - 3 \\
4 = \frac{4}{p} \\
4t = \frac{4}{p^2} \\
5 g(p) = f(p) (p - 4) - \frac{4}{p} \\
f(p) = \frac{19 p^2 + 16 p + 20}{p^2(p^2 + 4)} = 
A \frac{1}{p} + B \frac{1}{p^2} + C \frac{p}{p^2 + 4} + D \frac{1}{p^2 + 4} \\
A = 4, \quad B = 5, \quad C = -4, \quad D = 14 \\
x = 4 + 5t - 4\cos{2t} + 7 \sin{2t} \\
g(p) = -\frac{3}{p} -\frac{4}{p^2} + \frac{6p - 8}{p^2 + 4} \\
y = -3 - 4t + 6 \cos{2t} - 4 \sin{2t}
} \\
$$
