---
id: 1733321768-уравнение-Лагранжа
aliases:
  - уравнение Лагранжа
tags: []
---

# уравнение Лагранжа
$$
\alignleft{
\sum_i{\veccross{R_i}{\delta r_i}} = 0 \\
m_i W_i = R_i + F_i \\
\sum_i{m_i \veccross{W_i}{\delta r_i}} = 
\sum_{k}{\left(\Dv{t}{\dv{\dot{{q}_{k}}}{T}} - \dv{q_k}{T}\right) \delta q_k} \\
\delta r_i = \sum_k{\dv{q_k}{r_i} \delta q_k} \\
\sum_i{\veccross{F_i}{\delta r_i}} = 
\sum_k{\delta q_k \sum_i{\veccross{F_i}{\dv{q_k}{r_i}}}} \\
Q_k = \sum_i{\veccross{F_i}{\dv{q_k}{r_i}}}\\
\sum_{k}{\left(\Dv{t}{\dv{\dot{{q}_{k}}}{T}} - \dv{q_k}{T} - Q_k\right) \delta q_k} = 0\\
}
$$
$$
\Dv{t}{\dv{\dot{{q}_{k}}}{T}} - \dv{q_k}{T} = Q_k, \quad \forall k
$$
$T$ - ***кинетическая энергия***
$Q_k = \sum_{i}{F_i \dv{q_k}{r_i}}$ - ***обобщенные силы***
$F_i$ - ***активные силы***
$q_k$ - ***параметризация системы***
##
`Let:` $F$ - [[1728729433-потенциальная-сила|потенциальная сила]]
$$
\alignleft{
Q_k = \sum_k{\veccross{F_i}{\dv{q_k}{r_i}}} =
\sum_k{\veccross{-\dv{r_i}{\Pi}}{\dv{q_k}{r_i}}} =
-\dv{q_k}{\Pi} \\
Q_k = Q_k^{pot} + Q_k^{npot} \\
}
$$
$$
\Gather{
L = T - \Pi \\
\Dv{t}{\dv{\dot{{q}_{k}}}{L}} - \dv{q_k}{L} = Q_k^{npot}, \quad \forall k
}
$$
## Ковариантность
## 
$L \sim L(q, \dot{q}, t) + \Dv{t}{F(q,t)}$
## Структуры кин. энергии
$T \defeq \frac{1}{2} \int{v^2 \d m}$
$v = \dot{r} = \dv{t}{r} t + \sum_{k}{\dv{q_k}{r} \dot{q_k}}$ 
$T = T_2 + T_1 + T_0$
$T = \frac{1}{2} \sum_{i,j}{a_{ij} \dot{q_i}\dot{q_j}} + \sum_{i}{b_i \dot{{q}_{i}}} + b$ 
#
$$\Dv{t}{\dv{\dot{q}}{L}} - \dv{q}{L} = 0$$
## Циклические переменные
$q: \dv{q}{L} = 0$
$\Dv{t}{\dv{\dot{q}}{L}} = 0 \implies$
$\dv{\dot{q}}{L}$ - [[1729330322-первый-интеграл-движения|первый интеграл движения]]
## Обобщенный интеграл движения
$\dv{t}{L} = \dv{t}{L} \dot{t} + \dv{q}{L} \dot{q} + \dv{\dot{q}}{L} \ddot{q}$
##
$p = \dv{\dot{q}}{L}$ - обобщенный импульс
$H(q,p,t) = q \dot{q} - L(q, \dot{q}, t)$ 
$\dv{q}{H} = \dv{q}{L} = \dot{p}$
$\dv{p}{H} = \dot{q}$
***Уравнения Гамильтона***
$$
\aligncenter{
\dot{q} = \dv{p}{H} \\
\dot{p} = -\dv{q}{H}
}
$$
$(q,p) \to ({q}^{'}, {p}^{'}) : {H}^{'} = 0$
$p = const, q = at + b$
