---
id: 568-mipt-differential-equations-seminar-09-04-25
aliases:
  - MIPT differential equations seminar 09-04-25
tags: []
---

# MIPT differential equations seminar 09-04-25

![задачи.png](assets/imgs/09-04-25_15-56-53_914_09-04-25_15-56-53_062.png)

# Theory

![.jpg](assets/imgs/09-04-25_16-07-02_355_IMG_20250409_160504.jpg)

# T1

У доски.

# Р 14.12

![14-12.png](assets/imgs/09-04-25_15-59-19_990_09-04-25_15-59-19_141.png)

$\Align{
\hline
1.\ a = 0 \\
\Cases{
\dot{x} = y \\
\dot{y} = -x
} \\
(x_0, y_0) = (0,0) - ПР \\
\lambda_{1,2} = \pm i \\
\textit{Центр, по часовой.} \\
\frac{\d x}{y} = - \frac{\d y}{x} \\
u = x^2 + y^2 - ПИ \\
\hline
2.\ a \neq 0 \\
(x_0, y_0) = (0,0) - ПР \\
\Cases{
x = \rho \cos\varphi \\
y = \rho\sin\varphi
} \\
\Cases{
\dot{\rho} = a \rho (\rho^2 - 2) \\
\dot{\varphi} = -1 \\
}
\textit{Фокусы.}
}$
![.jpg](assets/imgs/09-04-25_16-18-59_715_IMG_20250409_161835.jpg)

# 1164

![1164.png](assets/imgs/09-04-25_16-21-30_449_09-04-25_16-21-30_649.png)

$\Align{
\grad u_1 = \frac{1}{(z+x)^2} \Pmatrix{
z-y \\
z + x \\
-x - y
} \\
\grad u_2 = \frac{1}{(x+y)^2} \Pmatrix{
-z+y \\
-x-z \\
x+y
} \\
\textit{В каждой точке линейно зависимы.} \\
}$

# T2.a

$\Align{
\Cases{
\dot{x} = y \\
\dot{y} = -\sin x
} \\
(x_0, y_0) = (\pi k,0) - ПР \\
\frac{\d x}{y} = -\frac{\d y}{\sin x} \\
u = 2 \cos x - y^2 = C - ПИ \\
}$

# Р 16.6

![.png](assets/imgs/09-04-25_16-40-06_831_09-04-25_16-40-06_548.png)
![.png](assets/imgs/09-04-25_16-40-35_455_09-04-25_16-40-35_584.png)

$\Align{
u_1 = x + y = C_1 \\
\dot{x} - x (1-C_1) = x^2
}$
[[1729012183-ду-Бернулли|ДУ Бернули]]
$\Align{
x = \frac{1}{C_2 e^{(C_1 - 1) t} + \frac{1}{C_1 - 1}} \\
y = C_1 - \frac{1}{C_2 e^{(C_1 - 1) t} + \frac{1}{C_1 - 1}}
}$

# Р 16.26

![.png](assets/imgs/09-04-25_16-52-23_529_09-04-25_16-52-23_916.png)
![.png](assets/imgs/09-04-25_16-52-05_320_09-04-25_16-52-05_639.png)

$\Align{
\frac{\d x}{x^2} = \frac{\d y}{2x^3-xy-z} = \frac{\d z}{xz-2x^4} \\
\frac{\d x}{x} = \frac{\d(z + x^3)}{z + x^3} \\
r_1 = \frac{x}{z + x^3} - ПИ \\
}$
Второй ПИ не нашли...

Семинар [[693-mipt-differential-equations-seminar-16-04-25|16-04-25]].

$\Align{
\frac{\d x}{x^2} = \frac{\d y}{2 x^3 - xy - z} = \frac{\d z}{xz - 2x^4} \\
\d (xy) = \d z \\
u_2
}$
