---
id: 693-mipt-differential-equations-seminar-16-04-25
aliases:
  - MIPT differential equations seminar 16-04-25
tags: []
---

# MIPT differential equations seminar 16-04-25

![16-04-25_15-49-51_672.png](assets/imgs/16-04-25_15-49-51_672.png)

# 17.4

![16-04-25_15-51-00_229.png](assets/imgs/16-04-25_15-51-00_229.png)
![16-04-25_15-51-13_894.png](assets/imgs/16-04-25_15-51-13_894.png)

$\Align{
\Cases{
\dot{x} = x^2 + z^2 \\
\dot{y} = 2(xy - xz^3) \\
\dot{z} = 2xz
} \\
(1)\ Ð¸\ (2) \\
\frac{\d x}{x^2 + z^2} = \frac{\d y}{2(xy - xz^3)} = \frac{\d z}{2xz} \\
\frac{\d (x+z)}{(x+z)^2} = \frac{\d (x-z)}{(x-z)^2} \\
\frac{1}{x + z} = \frac{1}{x - z} + C \\
u_1 = \frac{z}{x^2 + z^2}
}$
